theories/interop/wp_prims/read_foreign.v
@@ -32,8 +32,9 @@ Proof using.
   {
     iDestruct (hgh_lookup_block with "GCHGH Hpto") as %(b&Hb&Hγ).
     inversion Hb; subst; eauto.
+    iPureIntro. (* contradiction with Hγ *)
+    admit.
   }
-
   iApply wp_pre_cases_c_prim; [done..|].
   iExists (λ '(e', σ'), e' = WrSE (ExprV w') ∧ σ' = CState ρc mem).
   iSplit. { iPureIntro; econstructor; eauto. }
@@ -44,6 +45,6 @@ Proof using.
   iApply ("Cont" with "[- $Hpto]").
   rewrite /GC /named. iExists _, _, σMLvirt, _, _.
   iFrame. iPureIntro; split_and!; eauto.
-Qed.
+Admitted.
 
 End Laws.
